stuff

Cons.v
@@ -1,6 +1,8 @@
 Require Import DataTypes.
 Require Import List.
 
+Set Implicit Arguments.
+
 Definition Tag := nat.
 
 Inductive Req :=
@@ -19,15 +21,15 @@ Inductive Inst :=
 | St: Addr -> Data -> Inst.
 
 Section PerProc.
-  Parameter Pc: Set.
-  Parameter State: Set.
-  Parameter DeltaState: Set.
+  Variable Pc: Set.
+  Variable State: Set.
+  Variable DeltaState: Set.
 
-  Parameter nextSt: Pc -> option Data -> (Pc * Inst * DeltaState).
-  Parameter updSt: State -> DeltaState -> State.
+  Variable nextSt: Pc -> option Data -> (Pc * Inst * DeltaState).
+  Variable updSt: State -> DeltaState -> State.
 
   Inductive Normal: State -> Pc -> list Req -> list Resp -> bool ->
-                    State -> Pc -> list Req -> list Resp -> bool -> Set :=
+                    State -> Pc -> list Req -> list Resp -> bool -> Prop :=
   | ComNonMem: forall s nextPc p2m m2p nextPc' delS,
                  nextSt nextPc None = (nextPc', Nm, delS) ->
                  Normal s nextPc p2m m2p false (updSt s delS) nextPc' p2m m2p false
@@ -50,8 +52,127 @@ Section PerProc.
       forall s nextPc p2m m2p x w,
         Normal s nextPc p2m (m2p ++ (x :: nil)) w s nextPc p2m m2p w.
 
-  Parameter Rob: Set.
+  Section NormalList.
+    Variable s0: State.
+    Variable n0: Pc.
+    Inductive NormalList:
+      State -> Pc -> list Req -> list Resp -> bool -> Prop :=
+    | InitNormal: NormalList s0 n0 nil nil false
+    | CreateNormal: forall s nextPc p2m m2p w s' nextPc' p2m' m2p' w',
+                      Normal s nextPc p2m m2p w s' nextPc' p2m' m2p' w' ->
+                      NormalList s nextPc p2m m2p w ->
+                      NormalList s' nextPc' p2m' m2p' w'.
+  End NormalList.
 
-  Inductive Spec: State -> Pc -> Rob -> list Req -> list Resp ->
-                  State -> Pc -> Rob -> list Req -> list Resp 
+  Variable Rob: Set.
+
+  Definition CommitEntry := (Pc * Pc * Inst * option Data * DeltaState)%type.
+
+  Variable enq: Pc -> Rob -> Rob.
+
+  Variable Ppc: Set.
+  Variable nextPpc: Ppc -> Ppc.
+  Variable execute: Rob -> Rob.
+  Variable getLoad: Rob -> option (Tag * Addr)%type.
+  Variable issueLoad: Tag -> Rob -> Rob.
+  Variable updLoad: Tag -> Data -> Rob -> Rob.
+  Variable getCommitPc: Rob -> option Pc.
+  Variable empty: Rob.
+  Variable setPpc: Pc -> Ppc.
+  Variable getCommitFull: Rob -> option CommitEntry.
+  Variable finishCommit: Rob -> Rob.
+
+  Inductive CommitState :=
+  | StCom: CommitState
+  | LdCom: Pc -> Addr -> Data -> DeltaState -> CommitState.
+
+  Inductive Spec:
+    State -> Pc -> list Req -> list Resp -> Rob ->
+    option (CommitState) -> Ppc ->
+    State -> Pc -> list Req -> list Resp -> Rob ->
+    option (CommitState) -> Ppc -> Set :=
+  | SpecNotLd: forall s nextPc p2m m2p rob nextCommit ppc,
+                 Spec s nextPc p2m m2p rob nextCommit ppc
+                      s nextPc p2m m2p (enq nextPc rob) nextCommit (nextPpc ppc)
+  | SpecExecute: forall s nextPc p2m m2p rob nextCommit ppc,
+                   Spec s nextPc p2m m2p rob nextCommit ppc
+                        s nextPc p2m m2p (execute rob) nextCommit ppc
+  | SpecLdReq:
+      forall s nextPc p2m m2p rob nextCommit ppc tag a,
+        getLoad rob = Some (tag, a) ->
+        Spec s nextPc p2m m2p rob nextCommit ppc
+             s nextPc (LdReq tag a :: p2m) m2p (issueLoad tag rob) nextCommit ppc
+  | SpecLdResp:
+      forall s nextPc p2m m2p rob nextCommit ppc tag v,
+        Spec s nextPc p2m (LdResp tag v :: m2p) rob nextCommit ppc
+             s nextPc p2m m2p (updLoad tag v rob) nextCommit ppc
+  | SpecAbort:
+      forall s nextPc p2m m2p rob ppc,
+        getCommitPc rob <> Some nextPc ->
+        Spec s nextPc p2m m2p rob None ppc
+             s nextPc p2m m2p empty None (setPpc nextPc)
+  | SpecComNm:
+      forall s nextPc p2m m2p rob ppc delS nextPc',
+        getCommitFull rob = Some (nextPc, nextPc', Nm, None, delS) ->
+        nextSt nextPc None = (nextPc', Nm, delS) ->
+        Spec s nextPc p2m m2p rob None ppc
+             (updSt s delS) nextPc' p2m m2p (finishCommit rob) None ppc
+  | SpecComStReq:
+      forall s nextPc p2m m2p rob ppc delS nextPc' a v,
+        getCommitFull rob = Some (nextPc, nextPc', St a v, None, delS) ->
+        nextSt nextPc None = (nextPc', St a v, delS) ->
+        Spec s nextPc p2m m2p rob None ppc
+             (updSt s delS) nextPc' (StReq a v :: p2m) m2p
+             (finishCommit rob) (Some StCom) ppc
+  | SpecComStResp:
+      forall s nextPc p2m m2p rob ppc,
+        Spec s nextPc p2m (StResp :: m2p) rob (Some StCom) ppc
+             s nextPc p2m m2p (finishCommit rob) None ppc
+  | SpecComLdReq:
+      forall s nextPc p2m m2p rob ppc delS nextPc' a v,
+        getCommitFull rob = Some (nextPc, nextPc', Ld a, Some v, delS) ->
+        Spec s nextPc p2m m2p rob None ppc
+             s nextPc (StReq a v :: p2m) m2p
+             (finishCommit rob) (Some (LdCom nextPc' a v delS)) ppc
+  | SpecComLdRespGood:
+      forall s nextPc p2m m2p rob ppc delS nextPc' a v,
+        nextSt nextPc (Some v) = (nextPc', Ld a, delS) ->
+        Spec s nextPc p2m (LdCommitResp v :: m2p) rob (Some (LdCom nextPc' a v delS)) ppc
+             (updSt s delS) nextPc' p2m m2p (finishCommit rob) None ppc
+  | SpecComLdRespBad:
+      forall s nextPc p2m m2p rob ppc delS nextPc' a v v' delS',
+        nextSt nextPc (Some v') = (nextPc', Ld a, delS') ->
+        Spec s nextPc p2m (LdCommitResp v' :: m2p) rob (Some (LdCom nextPc' a v delS)) ppc
+             (updSt s delS') nextPc' p2m m2p (finishCommit rob) None ppc
+  | SpecExternalReq:
+      forall s nextPc p2m m2p x rob nextCommit ppc,
+        Spec s nextPc (p2m ++ (x :: nil)) m2p rob nextCommit ppc
+             s nextPc p2m m2p rob nextCommit ppc
+  | SpecExternalResp:
+      forall s nextPc p2m m2p x rob nextCommit ppc,
+        Spec s nextPc p2m (m2p ++ (x :: nil)) rob nextCommit ppc
+             s nextPc p2m m2p rob nextCommit ppc.
+
+  Section SpecList.
+    Variable s0: State.
+    Variable n0: Pc.
+    Variable ppc0: Ppc.
+    Inductive SpecList:
+      State -> Pc -> list Req -> list Resp -> Rob -> option CommitState -> Ppc -> Prop :=
+    | InitSpec: SpecList s0 n0 nil nil empty None ppc0
+    | CreateSpec:
+        forall s nextPc p2m m2p rob cs ppc s' nextPc' p2m' m2p' rob' cs' ppc',
+          Spec s nextPc p2m m2p rob cs ppc s' nextPc' p2m' m2p' rob' cs' ppc' ->
+          SpecList s nextPc p2m m2p rob cs ppc ->
+          SpecList s' nextPc' p2m' m2p' rob' cs' ppc'.
+  End SpecList.
+
+  Theorem specNormal:
+    forall s0 n0 ppc0 s nextPc p2m m2p rob cs ppc,
+      SpecList s0 n0 ppc0 s nextPc p2m m2p rob cs ppc ->
+      exists p2m' m2p' w,
+        NormalList s0 n0 s nextPc p2m' m2p' w.
+  Proof.
+    admit.
+  Qed.
 End PerProc.
